partial completion of cencode_not_equal_def and cencode_not_equal_sem

examples/pseudo_bool/cp_encoding/cp_to_ilp_primScript.sml
@@ -160,112 +160,53 @@ Proof
   intLib.ARITH_TAC
 QED
 
-(* this will encompass ≥, >, ≤, < *)
-Definition encode_other_cmpops_def:
-  encode_other_cmpops bnd Zr cmp X Y =
+(* this encompasses ≥, >, ≤, < *)
+Definition encode_order_cmpops_def:
+  encode_order_cmpops bnd Zr cmp X Y =
   let constr =
     (case cmp of
       GreaterEqual => mk_constraint_ge 1 X (-1) Y 0
     | GreaterThan  => mk_constraint_ge 1 X (-1) Y 1
     | LessEqual    => mk_constraint_ge (-1) X 1 Y 0
     | LessThan     => mk_constraint_ge (-1) X 1 Y 1
-    | _            => ARB)
+    | _            => false_constr)
   in
-    if (cmp = Equal ∨ cmp = NotEqual)
-    then [([],[],0i)]
-    else
-      case Zr of
-        NONE => [constr]
-      | SOME (INL Z) =>
-        encode_ge bnd Z 1 ++
-        [bits_imply bnd [Pos (INL (Ge Z 1))] constr]
-      | SOME (INR Z) =>
-        encode_ge bnd Z 1 ++
-        bimply_bits bnd [Pos (INL (Ge Z 1))] constr
+    case Zr of
+      NONE => [constr]
+    | SOME (INL Z) =>
+      encode_ge bnd Z 1 ++
+      [bits_imply bnd [Pos (INL (Ge Z 1))] constr]
+    | SOME (INR Z) =>
+      encode_ge bnd Z 1 ++
+      bimply_bits bnd [Pos (INL (Ge Z 1))] constr
 End
 
-(* to be deprecated *)
-Definition encode_greater_equal_def:
-  encode_greater_equal bnd Zr X Y =
-  let constr = mk_constraint_ge 1 X (-1) Y 0 in
-  case Zr of
-    NONE => [constr]
-  | SOME (INL Z) =>
-    encode_ge bnd Z 1 ++
-    [bits_imply bnd [Pos (INL (Ge Z 1))] constr]
-  | SOME (INR Z) =>
-    encode_ge bnd Z 1 ++
-    bimply_bits bnd [Pos (INL (Ge Z 1))] constr
-End
-
-(* to be deprecated *)
-Theorem encode_greater_equal_sem_1:
-  valid_assignment bnd wi ∧
-  reify_sem Zr wi
-    (varc wi X ≥ varc wi Y) ⇒
+Theorem encode_order_cmpops_sem_1:
+  valid_assignment bnd wi ∧ cmp ≠ Equal ∧ cmp ≠ NotEqual ∧
+  reify_sem Zr wi (cmpop_val cmp (varc wi X) (varc wi Y)) ⇒
   EVERY (λx. iconstraint_sem x (wi,reify_avar cs wi))
-    (encode_greater_equal bnd Zr X Y)
+    (encode_order_cmpops bnd Zr cmp X Y)
 Proof
-  rw[reify_sem_def,encode_greater_equal_def]>>
+  Cases_on ‘cmp’>>
+  rw[reify_sem_def,cmpop_val_def,
+    encode_order_cmpops_def,
+    iconstraint_sem_def]>>
+  every_case_tac>>
   gvs[AllCasePreds(),reify_avar_def,reify_reif_def]>>
   intLib.ARITH_TAC
 QED
 
-(* to be deprecated *)
-Theorem encode_greater_equal_sem_2:
-  valid_assignment bnd wi ∧
+Theorem encode_order_cmpops_sem_2:
+  valid_assignment bnd wi ∧ cmp ≠ Equal ∧ cmp ≠ NotEqual ∧
   EVERY (λx. iconstraint_sem x (wi,wb))
-    (encode_greater_equal bnd Zr X Y) ⇒
-  reify_sem Zr wi
-    (varc wi X ≥ varc wi Y)
+    (encode_order_cmpops bnd Zr cmp X Y) ⇒
+  reify_sem Zr wi (cmpop_val cmp (varc wi X) (varc wi Y))
 Proof
-  rw[reify_sem_def,encode_greater_equal_def]>>
+  rw[reify_sem_def,encode_order_cmpops_def,cmpop_val_def]>>
   every_case_tac>>
   gvs[]>>
   intLib.ARITH_TAC
 QED
-
-(* to be deprecated *)
-Definition encode_greater_than_def:
-  encode_greater_than bnd Zr X Y =
-  let constr = mk_constraint_ge 1 X (-1) Y 1 in
-  case Zr of
-    NONE => [constr]
-  | SOME (INL Z) =>
-    encode_ge bnd Z 1 ++
-    [bits_imply bnd [Pos (INL (Ge Z 1))] constr]
-  | SOME (INR Z) =>
-    encode_ge bnd Z 1 ++
-    bimply_bits bnd [Pos (INL (Ge Z 1))] constr
-End
-
-(* to be deprecated *)
-Definition encode_less_equal_def:
-  encode_less_equal bnd Zr X Y =
-  let constr = mk_constraint_ge (-1) X 1 Y 0 in
-  case Zr of
-    NONE => [constr]
-  | SOME (INL Z) =>
-    encode_ge bnd Z 1 ++
-    [bits_imply bnd [Pos (INL (Ge Z 1))] constr]
-  | SOME (INR Z) =>
-    encode_ge bnd Z 1 ++
-    bimply_bits bnd [Pos (INL (Ge Z 1))] constr
-End
-
-(* to be deprecated *)
-Definition encode_less_than_def:
-  encode_less_than bnd Zr X Y =
-  let constr = mk_constraint_ge (-1) X 1 Y 1 in
-  case Zr of
-    NONE => [constr]
-  | SOME (INL Z) =>
-    encode_ge bnd Z 1 ++
-    [bits_imply bnd [Pos (INL (Ge Z 1))] constr]
-  | SOME (INR Z) =>
-    encode_ge bnd Z 1 ++
-    bimply_bits bnd [Pos (INL (Ge Z 1))] constr
-End
 
 Definition encode_negative_def:
   encode_negative X Y =
@@ -289,13 +230,11 @@ Definition encode_prim_constr_def:
   encode_prim_constr bnd c name =
   case c of
     Cmpop Zr cmp X Y =>
-      (case cmp of
-        Equal => encode_equal bnd Zr X Y name
-      | NotEqual => encode_not_equal bnd Zr X Y name
-      | GreaterEqual => encode_greater_equal bnd Zr X Y
-      | GreaterThan => encode_greater_than bnd Zr X Y
-      | LessEqual => encode_less_equal bnd Zr X Y
-      | LessThan => encode_less_than bnd Zr X Y)
+      if cmp = Equal
+      then encode_equal bnd Zr X Y name
+      else if cmp = NotEqual
+      then encode_not_equal bnd Zr X Y name
+      else encode_order_cmpops bnd Zr cmp X Y
   | _ => ARB
 End
 
@@ -310,13 +249,12 @@ Proof
   rw[encode_prim_constr_def,prim_constr_sem_def]
   >- cheat
   >- cheat
-  >- (
-    gvs[cmpop_sem_def]>>
-    every_case_tac>>
-    gvs[cmpop_val_def]
-    >- metis_tac[encode_equal_sem_1]
-    >- metis_tac[encode_not_equal_sem_1]
-    >> cheat)
+  >- (irule encode_equal_sem_1>>
+      gvs[cmpop_sem_def,cmpop_val_def])
+  >- (irule encode_not_equal_sem_1>>
+      gvs[cmpop_sem_def,cmpop_val_def])
+  >> (irule encode_order_cmpops_sem_1>>
+      gvs[cmpop_sem_def,cmpop_val_def])
 QED
 
 Theorem encode_prim_constr_sem_2:
@@ -328,12 +266,131 @@ Proof
   rw[encode_prim_constr_def,prim_constr_sem_def]
   >- cheat
   >- cheat
-  >- (
-    gvs[cmpop_sem_def]>>
-    every_case_tac>>
-    gvs[cmpop_val_def]
-    >- metis_tac[encode_equal_sem_2]
-    >- metis_tac[encode_not_equal_sem_2]
-    >> cheat)
+  >- (gvs[cmpop_sem_def,cmpop_val_def]>>
+      metis_tac[encode_equal_sem_2])
+  >- (gvs[cmpop_sem_def,cmpop_val_def]>>
+      metis_tac[encode_not_equal_sem_2])
+  >- (gvs[cmpop_sem_def]>>
+      metis_tac[encode_order_cmpops_sem_2])
 QED
 
+Definition cencode_equal_def:
+  cencode_equal bnd Zr X Y name ec =
+  let constr =
+    [
+      (SOME (strlit "ge"),mk_constraint_ge 1 (X) (-1) (Y) 0);
+      (SOME (strlit "le"),mk_constraint_ge 1 (Y) (-1) (X) 0)
+    ] in
+  case Zr of
+    NONE => (List constr,ec)
+  | SOME (INL Z) =>
+      let
+        (e,ec') = cencode_ge bnd Z 1 ec
+      in
+        (Append e $
+          List (MAP (I ## bits_imply bnd [Pos (INL (Ge Z 1))]) constr),ec')
+  | SOME (INR Z) =>
+      let
+        (e,ec') = cencode_ge bnd Z 1 ec
+      in
+        (Append e $
+          List (
+          MAP (I ## bits_imply bnd [Pos (INL (Ge Z 1))]) constr ++
+          [
+            (SOME (strlit "gt"),bits_imply bnd [Pos (gt_var name)]
+              (mk_constraint_ge 1 X (-1) Y 1));
+            (SOME (strlit "lt"),bits_imply bnd [Pos (lt_var name)]
+              (mk_constraint_ge 1 Y (-1) X 1));
+            (SOME (strlit "al1"),at_least_one
+              [
+                Pos (lt_var name); Pos (gt_var name);
+                Pos (INL (Ge Z 1))
+              ]);
+          ]),ec')
+End
+
+Theorem enc_rel_List_refl_mul:
+  set ls' = set $ MAP SND ls ⇒
+  enc_rel wi (List ls) ls' ec ec
+Proof
+  rw[enc_rel_def]>>
+  fs[EVERY_MEM,EXTENSION,MEM_MAP]>>
+  metis_tac[]
+QED
+
+Theorem cencode_equal_sem:
+  valid_assignment bnd wi ∧
+  cencode_equal bnd Zr X Y name ec = (es, ec') ⇒
+  enc_rel wi es (encode_equal bnd Zr X Y name) ec ec'
+Proof
+  rw[cencode_equal_def,encode_equal_def]>>
+  gvs[AllCaseEqs(),UNCURRY_EQ]
+  >- simp[enc_rel_List_refl_mul]
+  >- (
+    irule enc_rel_Append>>
+    irule_at Any enc_rel_encode_ge>>
+    simp[enc_rel_List_refl_mul])
+  >> (
+    pure_rewrite_tac[GSYM APPEND_ASSOC]>>
+    irule enc_rel_Append>>
+    irule_at Any enc_rel_encode_ge>>
+    simp[enc_rel_List_refl_mul])
+QED
+
+(* HERE *)
+Definition cencode_not_equal_def:
+  cencode_not_equal bnd Zr X Y name ec =
+  let xgty = (mk_constraint_ge 1 X (-1) Y 1) in
+  let ygtx = (mk_constraint_ge 1 Y (-1) X 1) in
+    case Zr of
+      NONE =>
+      (List
+        [
+          (SOME (strlit "gt"),bits_imply bnd [Pos (ne_var name)] xgty);
+          (SOME (strlit "lt"),bits_imply bnd [Neg (ne_var name)] ygtx)
+        ],ec)
+    | SOME (INL Z) =>
+        let
+          (e,ec') = cencode_ge bnd Z 1 ec
+        in
+          (Append e $
+            List $
+              (MAP (λc. (SOME (strlit "gt"),c)) $
+                bimply_bits bnd [Pos (gt_var name)] xgty) ++
+              (MAP (λc. (SOME (strlit "lt"),c)) $
+                bimply_bits bnd [Pos (lt_var name)] ygtx) ++
+              [
+               (SOME (strlit "al1"),at_least_one
+                 [
+                   Pos (lt_var name);
+                   Pos (gt_var name);
+                   Neg (INL (Ge Z 1))
+                 ])
+              ],ec')
+  (*
+  | SOME (INR Z) =>
+    encode_ge bnd Z 1 ++
+    MAP (bits_imply bnd [Neg (INL (Ge Z 1))])
+      [
+        mk_constraint_ge 1 (X) (-1) (Y) 0;
+        mk_constraint_ge 1 (Y) (-1) (X) 0
+      ] ++
+    [
+      bits_imply bnd [Pos (gt_var name)] xgty;
+      bits_imply bnd [Pos (lt_var name)] ygtx;
+      at_least_one
+        [Pos (lt_var name); Pos (gt_var name);
+          Neg (INL (Ge Z 1))];
+    ]*)
+End
+
+Theorem cencode_not_equal_sem:
+  valid_assignment bnd wi ∧
+  cencode_not_equal bnd Zr X Y name ec = (es, ec') ⇒
+  enc_rel wi es (encode_not_equal bnd Zr X Y name) ec ec'
+Proof
+  rw[cencode_not_equal_def,encode_not_equal_def]>>
+  gvs[AllCaseEqs(),UNCURRY_EQ]
+  >- simp[enc_rel_List_refl_mul]
+  >> cheat
+QED
